Syntax.v
@@ -1858,6 +1858,7 @@ Proof.
     apply (inlineSingle f (a ty)).
 Defined.
 
+(* BaseModule version of inlineSingle_Rule done *)
 Definition inlineSingle_Rule_map_BaseModule (f : DefMethT) (m : BaseModule) :=
   BaseMod (getRegisters m) (map (inlineSingle_Rule f) (getRules m)) (getMethods m).
 
@@ -1870,7 +1871,7 @@ Fixpoint inlineSingle_Rule_in_list (f : DefMethT) (rn : string) (lr : list RuleT
   | nil => nil
   end.
 
-(* module version of inlineSingle_Rule_in_list *)
+(* BaseModule version of inlineSingle_Rule_in_list done *)
 Definition inlineSingle_Rule_BaseModule (f : DefMethT) (rn : string) (m : BaseModule) :=
   BaseMod (getRegisters m) (inlineSingle_Rule_in_list f rn (getRules m)) (getMethods m).
 
@@ -1889,6 +1890,7 @@ Proof.
       apply (inlineSingle f (m ty X)).
 Defined.
 
+(* BaseModule version of inlineSingle_Meth done *)
 Definition inlineSingle_Meth_map_BaseModule (f : DefMethT) (m : BaseModule) :=
   BaseMod (getRegisters m) (getRules m) (map (inlineSingle_Meth f) (getMethods m)).
 
@@ -1901,7 +1903,7 @@ Fixpoint inlineSingle_Meth_in_list (f : DefMethT) (gn : string) (lm : list DefMe
   | nil => nil
   end.
 
-(* module version of inlineSingle_Meth_in_list *)
+(* BaseModule version of inlineSingle_Meth_in_list done *)
 Definition inlineSingle_Meth_BaseModule (f : DefMethT) (fn : string) (m : BaseModule) :=
   BaseMod (getRegisters m) (getRules m) (inlineSingle_Meth_in_list f fn (getMethods m)).
 
@@ -1909,15 +1911,15 @@ Section inlineSingle_nth.
   Variable (f : DefMethT).
   Variable (regs: list RegInitT) (rules: list RuleT) (meths: list DefMethT).
 
-  (* Module version of both inlineSingle_Rule and inlineSingle_Meth *)
+  (* BaseModule version of both inlineSingle_Rule and inlineSingle_Meth done *)
   Definition inlineSingle_BaseModule : BaseModule :=
     BaseMod regs (map (inlineSingle_Rule f) rules) (map (inlineSingle_Meth f) meths).
 
-  (* Iterated module version of inlineSingle_Meth *)
+  (* Iterated BaseModule version of inlineSingle_Meth done *)
   Definition inlineSingle_BaseModule_nth_Meth xs : BaseModule :=
     BaseMod regs rules (fold_right (transform_nth_right (inlineSingle_Meth f)) meths xs).
 
-  (* Iterated module version of inlineSingle_Rule *)
+  (* Iterated BaseModule version of inlineSingle_Rule done *)
   Definition inlineSingle_BaseModule_nth_Rule xs : BaseModule :=
     BaseMod regs (fold_right (transform_nth_right (inlineSingle_Rule f)) rules xs) meths.
 End inlineSingle_nth.
@@ -1930,6 +1932,7 @@ Definition inlineSingle_Rules_pos meths n rules :=
 
 Definition inlineAll_Rules meths rules := fold_left (fun newRules n => inlineSingle_Rules_pos meths n newRules) (0 upto (length meths)) rules.
 
+(* BaseModule version of inlineAll_Rules done *)
 Definition inlineAll_Rules_mod m :=
   (BaseMod (getRegisters m) (inlineAll_Rules (getMethods m) (getRules m)) (getMethods m)).
 
@@ -1941,15 +1944,18 @@ Definition inlineSingle_Meths_pos newMeths n :=
 
 Definition inlineAll_Meths meths := fold_left inlineSingle_Meths_pos (0 upto (length meths)) meths.
 
+(* BaseModule version of inlineAll_Meths done *)
 Definition inlineAll_Meths_mod m :=
   (BaseMod (getRegisters m) (getRules m) (inlineAll_Meths (getMethods m))).
 
 Definition inlineAll_All regs rules meths :=
   (BaseMod regs (inlineAll_Rules (inlineAll_Meths meths) rules) (inlineAll_Meths meths)).
 
+(* BaseModule version of inlineAll_All done *)
 Definition inlineAll_All_mod m :=
   inlineAll_All (getAllRegisters m) (getAllRules m) (getAllMethods m).
 
+(* Module version of inlineAll_All done *)
 Definition flatten_inline_everything m :=
   createHide (inlineAll_All_mod m) (getHidden m).
 
@@ -1957,6 +1963,7 @@ Definition removeHides (m: BaseModule) s :=
   BaseMod (getRegisters m) (getRules m)
           (filter (fun df => negb (getBool (in_dec string_dec (fst df) s))) (getMethods m)).
 
+(* BaseModule of inlineAll_All which removes initially hidden methods *)
 Definition flatten_inline_remove m :=
   removeHides (inlineAll_All_mod m) (getHidden m).
   
